code/mpfr/MPFR.Sub1.Spec.fst
@@ -1,0 +1,62 @@
+module MPFR.Sub1.Spec
+
+open FStar.Mul
+open MPFR.Dyadic
+open MPFR.Lib.Spec
+open MPFR.Maths
+
+#set-options "--z3refresh --z3rlimit 15 --max_fuel 1 --initial_fuel 0 --max_ifuel 1 --initial_ifuel 0"
+
+(* In this specification we only consider MPFR normal numbers as input *)
+
+(* Useful functions when subtracting two MPFR numbers with same precision
+ * and the first one is greater than that the second one *)
+val sub1sp_gt_limb: a:mpfr_reg_fp ->
+    b:mpfr_reg_fp{a.prec = b.prec /\ a.exp >= b.exp /\ (gt (eval_abs a) (eval_abs b))} ->
+    Tot (rm:pos{rm =(eval_abs a -. eval_abs b).significand})
+
+let sub1sp_gt_limb a b =
+    //! assert((a.limb * pow2 (a.exp - b.exp) - b.limb) = (eval_abs a -. eval_abs b).significand);
+    lemma_mul_mod_zero a.limb (pow2 (a.exp - b.exp)) (pow2 (a.len - a.prec));
+    a.limb * pow2 (a.exp - b.exp) - b.limb
+
+val sub1sp_gt_len: a:mpfr_reg_fp -> 
+    b:mpfr_reg_fp{a.prec = b.prec /\ a.exp >= b.exp /\ (gt (eval_abs a) (eval_abs b))} ->
+    Tot (rl:pos{sub1sp_gt_limb a b >= pow2 (rl - 1) /\ sub1sp_gt_limb a b < pow2 rl})
+
+let sub1sp_gt_len a b =
+    lemma_pow2_nbits (sub1sp_gt_limb a b);
+    nbits  (sub1sp_gt_limb a b)
+
+let sub1sp_gt_exp a b =
+    b.exp + sub1sp_gt_len a b - b.len
+
+let sub1sp_gt_prec a b =sub1sp_gt_len a b
+
+(* Subtraction for two MPFR numbers with same precision *)
+val sub1sp_exact: a:mpfr_reg_fp ->
+    b:mpfr_reg_fp{a.prec = b.prec} ->
+    Tot (r:valid_fp{((gt (eval_abs a) (eval_abs b) /\ r.sign = a.sign) \/
+                    (eq (eval_abs a) (eval_abs b)) \/
+                    (lt (eval_abs a) (eval_abs b) /\ r.sign = -a.sign))
+                    /\ fabs (eval_abs a -. eval_abs b) =. eval_abs r})
+
+val lemma_fp_exp_ge: a:mpfr_reg_fp ->
+    b:mpfr_reg_fp -> Lemma
+    (requires (a.prec=b.prec /\ ge (eval_abs a) (eval_abs b)))
+    (ensures (a.exp>=b.exp))
+let lemma_fp_exp_ge a b=let elb=min (a.exp-a.len) (b.exp-b.len) in
+       assert(a.limb * pow2 (a.exp-a.len-elb)>=b.limb * pow2 (b.exp-b.len-elb));
+       //! assert(pow2 a.len * pow2 (a.exp-a.len-elb)>b.limb * pow2 (b.exp-b.len-elb));
+       assert(pow2 a.len * pow2 (a.exp-a.len-elb)>pow2 (b.len-1) * pow2 (b.exp-b.len-elb));
+       lemma_pow2_mul a.len (a.exp-a.len-elb);
+       assert(pow2 (a.exp-elb)>pow2 (b.len-1) * pow2 (b.exp-b.len-elb));
+       lemma_pow2_mul (b.len-1) (b.exp-b.len-elb);
+       assert(pow2 (a.exp-elb)>pow2 (b.exp-1-elb));
+       lemma_pow2_gt_rev (a.exp-elb) (b.exp-1-elb)
+
+let sub1sp_exact ar br = 
+    if eq (eval_abs ar) (eval_abs br) then mpfr_zero 1 1 else
+    let rs,a,b = if gt (eval_abs ar) (eval_abs br) then ar.sign,ar,br else -ar.sign,br,ar in
+       lemma_fp_exp_ge a b;
+       mk_fp_struct rs (sub1sp_gt_prec a b) (sub1sp_gt_exp a b) (sub1sp_gt_limb a b) (sub1sp_gt_len a b) MPFR_NUM
