code/mpfr/MPFR.Sub1sp1.fst
@@ -1,0 +1,202 @@
+module MPFR.Sub1sp1
+
+open FStar.HyperStack.All
+open FStar.HyperStack
+open FStar.HyperStack.ST
+open FStar.Buffer
+open FStar.UInt64
+open FStar.Int.Cast
+open FStar.Mul
+open MPFR.Dyadic
+open MPFR.Lib.Spec
+open MPFR.Sub1.Spec
+open MPFR.Round.Spec
+open MPFR.Maths
+
+open MPFR.Lib
+open MPFR.Exceptions
+
+open MPFR.Exceptions.Lemma
+(*open MPFR.Sub1sp1.Lemma*)
+
+module ST = FStar.HyperStack.ST
+module I32 = FStar.Int32
+module I64 = FStar.Int64
+module U32 = FStar.UInt32
+
+#set-options "--z3refresh --z3rlimit 100 --max_fuel 1 --initial_fuel 0 --max_ifuel 1 --initial_ifuel 0"
+
+private type mpfr_tmp_exp_t = x:mpfr_exp_t{I64.(x >=^ mpfr_EMIN /\ x <=^ mpfr_EMAX +^ 1L)}
+
+private noeq type state = {
+    sh:mpfr_reg_prec_t;
+    bx:mpfr_tmp_exp_t;
+    rb:mp_limb_t;
+    sb:mp_limb_t
+}
+
+let mk_state sh bx rb sb = {
+    sh = sh;
+    bx = bx;
+    rb = rb;
+    sb = sb
+}
+
+let mpfr_sub1sp1_pre_cond h (a:mpfr_ptr) b c (p:mpfr_prec_t): GTot Type0=
+        (* Memory safety *)
+        mpfr_live h a /\ mpfr_live h b /\ mpfr_live h c /\
+        mpfr_disjoint_or_equal h a b /\ mpfr_disjoint_or_equal h a c /\
+        mpfr_disjoint_or_equal h b c /\
+        length (as_struct h a).mpfr_d = 1 /\
+        length (as_struct h b).mpfr_d = 1 /\ length (as_struct h c).mpfr_d = 1 /\
+        (* Functional correctness *)
+        I64.v p > 0 /\ I64.v p < 64 /\ p = (as_struct h a).mpfr_prec /\
+        p = (as_struct h b).mpfr_prec /\ p = (as_struct h c).mpfr_prec /\
+        (as_struct h a).mpfr_sign = (as_struct h b).mpfr_sign /\
+        mpfr_valid_cond h a /\ mpfr_reg_cond h b /\ mpfr_reg_cond h c
+
+let mpfr_sub1sp1_pre_cond_2 h (a:mpfr_ptr) b c bx cx ap bp cp: GTot Type0=
+ (as_struct h b).mpfr_exp=bx /\
+ (as_struct h c).mpfr_exp=cx /\ 
+ equal h (as_struct h a).mpfr_d h ap /\
+ equal h (as_struct h b).mpfr_d h bp /\
+ equal h (as_struct h c).mpfr_d h cp /\
+ live h ap /\ live h bp /\ live h cp
+
+let mpfr_sub1sp1_post_cond h0 t h1 (a:mpfr_ptr) b c (p:mpfr_reg_prec_t) rnd_mode exact: GTot Type0=
+        (* Memory safety *)
+        mpfr_live h1 a /\ mpfr_live h1 b /\ mpfr_live h1 c /\
+        mpfr_disjoint_or_equal h1 a b /\ mpfr_disjoint_or_equal h1 a c /\
+        mpfr_disjoint_or_equal h1 b c /\ mpfr_modifies a h0 h1 /\
+        (* Functional correctness *)
+        mpfr_valid_cond h1 a /\ 
+        mpfr_round_cond exact (I64.v p) rnd_mode (as_fp h1 a) /\
+        mpfr_ternary_cond (I32.v t) exact (as_fp h1 a)
+
+let mpfr_sub1sp1_round_spec (high:normal_fp) (rb:bool) (sb:bool) (rnd_mode:mpfr_rnd_t):
+    Tot (r:normal_fp{r.prec = high.prec}) =
+    if rb = false && sb = false then high
+    else if MPFR_RNDN? rnd_mode then begin
+	if rb = false || (sb = false && is_even high)
+	then high
+	else add_one_ulp high
+    end else if mpfr_IS_LIKE_RNDZ rnd_mode (high.sign < 0) then high
+    else add_one_ulp high
+
+inline_for_extraction val count_leading_zeros: a:u64{not (a=^0uL)}->Tot (cnt:u32{U32.v cnt<32})
+
+let  count_leading_zeros a=admit()
+
+inline_for_extraction val mpfr_sub1sp1_round:(*Warning : the ensure part is too copy-pasted to be correct*)
+    a:mpfr_ptr -> ap:buffer mp_limb_t -> sh:mpfr_reg_prec_t -> bx:mpfr_reg_exp_t ->
+    rb:mp_limb_t -> sb:mp_limb_t -> rnd_mode:mpfr_rnd_t ->Stack i32
+    (requires (fun h->True))
+    (ensures (fun h0 r h1-> mpfr_live h1 a /\ mpfr_modifies a h0 h1 /\ mpfr_valid_cond h1 a /\ True))
+
+let mpfr_sub1sp1_round a ap bx rb sb rnd_mode=admit()
+
+inline_for_extraction val mpfr_sub1sp1_eq_branch_1:
+    a:mpfr_ptr -> b:mpfr_ptr -> c:mpfr_ptr ->
+    ap:buffer mp_limb_t -> bp:buffer mp_limb_t -> cp:buffer mp_limb_t ->
+    bx:mpfr_reg_exp_t ->cx:mpfr_reg_exp_t
+    ->rnd_mode:mpfr_rnd_t->
+    p:mpfr_reg_prec_t -> sh:mpfr_reg_prec_t -> Stack i32
+    (requires (fun h->mpfr_sub1sp1_pre_cond h a b c p /\
+    mpfr_sub1sp1_pre_cond_2 h a b c bx cx ap bp cp /\
+    I64.(bx=^cx) /\ as_val h bp=as_val h cp 
+    ))
+ (ensures (fun h0 t h1 -> 
+   let exact=sub1sp_exact (as_fp h0 b) (as_fp h0 c) in 
+   mpfr_sub1sp1_post_cond h0 t h1 a b c p rnd_mode exact))
+
+let mpfr_sub1sp1_eq_branch_1 a b c ap bp cp bx cx rnd_mode p sh=
+    if rnd_mode=MPFR_RNDD then mpfr_SET_NEG a else mpfr_SET_POS a;
+    mpfr_SET_ZERO a;
+    mpfr_RET 0l
+
+inline_for_extraction val mpfr_sub1sp1_eq:
+    a:mpfr_ptr -> b:mpfr_ptr -> c:mpfr_ptr ->
+    ap:buffer mp_limb_t -> bp:buffer mp_limb_t -> cp:buffer mp_limb_t ->
+    bx:mpfr_reg_exp_t ->cx:mpfr_reg_exp_t
+    ->rnd_mode:mpfr_rnd_t->
+    p:mpfr_reg_prec_t -> sh:mpfr_reg_prec_t -> Stack i32
+    (requires (fun h-> mpfr_sub1sp1_pre_cond h a b c p /\
+    mpfr_sub1sp1_pre_cond_2 h a b c bx cx ap bp cp /\
+    I64.(bx=^cx)
+    ))
+    (ensures (fun h0 t h1->
+    let exact=sub1sp_exact (as_fp h0 b) (as_fp h0 c) in 
+    mpfr_sub1sp1_post_cond h0 t h1 a b c p rnd_mode exact))
+
+let mpfr_sub1sp1_eq a b c ap bp cp bx cx rnd_mode p sh =
+    if (bp.(0ul)=cp.(0ul)) then mpfr_sub1sp1_eq_branch_1 a b c ap bp cp bx cx rnd_mode p sh
+    else begin admit();
+       if(cp.(0ul)>^bp.(0ul)) then begin
+         //mpfr_SET_OPPOSITE_SIGN a b;
+         let a0=cp.(0ul) -^ bp.(0ul) in
+         let cnt=count_leading_zeros a0 in
+         ap.(0ul) <- a0<<^cnt;
+         mpfr_sub1sp1_round a ap bx 0uL 0uL rnd_mode
+       end else begin 
+         //mpfr_SET_SAME_SIGN a b;
+         let a0=bp.(0ul) -^ cp.(0ul) in
+         let cnt=count_leading_zeros a0 in
+         ap.(0ul) <- a0<<^cnt;
+         mpfr_sub1sp1_round a ap bx 0uL 0uL rnd_mode
+       end
+    end
+
+inline_for_extraction val mpfr_sub1sp1_gt:
+    a:mpfr_ptr -> b:mpfr_ptr -> c:mpfr_ptr ->
+    ap:buffer mp_limb_t -> bp:buffer mp_limb_t -> cp:buffer mp_limb_t ->
+    bx:mpfr_reg_exp_t ->cx:mpfr_reg_exp_t
+    ->rnd_mode:mpfr_rnd_t->
+    p:mpfr_reg_prec_t -> sh:mpfr_reg_prec_t -> Stack i32
+    (requires (fun h-> mpfr_live h a /\ mpfr_live h b /\ mpfr_live h c /\ length ap>0 /\ length bp>0 /\ length cp>0 /\ live h ap /\ live h bp /\ live h cp /\ I64.v sh = I64.v gmp_NUMB_BITS - I64.v p))
+    (ensures (fun h s h1->True))
+
+let mpfr_sub1sp1_gt a b c ap bp cp bx cx rnd_mode p sh =
+    let d = I64.(bx-^cx) in
+    let mask = mpfr_LIMB_MASK (int64_to_uint32 sh) in
+    admit()
+
+(* specifications for mpfr_sub1sp1 *)
+val mpfr_sub1sp1: a:mpfr_ptr -> b:mpfr_ptr -> c:mpfr_ptr ->
+                  rnd_mode:mpfr_rnd_t -> p:mpfr_prec_t -> Stack i32
+    (requires (fun h -> mpfr_sub1sp1_pre_cond h a b c p))
+    (ensures  (fun h0 t h1 ->
+    let exact=sub1sp_exact (as_fp h0 b) (as_fp h0 c) in
+    mpfr_sub1sp1_post_cond h0 t h1 a b c p rnd_mode exact))
+
+let mpfr_sub1sp1 a b c rnd_mode p =
+    let bx=mpfr_GET_EXP b in
+    let cx=mpfr_GET_EXP c in
+    let ap=mpfr_MANT a in
+    let bp=mpfr_MANT b in
+    let cp=mpfr_MANT c in
+    let sh=I64.(gmp_NUMB_BITS -^ p) in
+    if I64.(bx =^ cx) then mpfr_sub1sp1_eq a b c ap bp cp bx cx rnd_mode p sh else begin admit();
+   let bx,cx,bp,cp=(if I64.(bx >=^ cx) then (mpfr_SET_SAME_SIGN a b;bx,cx,bp,cp) else (mpfr_SET_OPPOSITE_SIGN a b;cx,bx,cp,bp)) in
+    ignore (mpfr_sub1sp1_gt a b c ap bp cp bx cx rnd_mode p sh);0l
+    end
+  (*  let st = mpfr_sub1sp1_any a b c ap p in()*)
+   (* let h1 = ST.get() in
+    lemma_reveal_modifies_1 (mpfr_MANT a) h0 h1;
+    lemma_intro_modifies_2 a (mpfr_MANT a) h0 h1;
+    if I64.(st.bx >^ mpfr_EMAX) then begin
+        let s = mpfr_SIGN a in
+        let t = mpfr_overflow a rnd_mode (mpfr_SIGN a) in
+	let h2 = ST.get() in
+	mpfr_overflow_post_cond_lemma (add1sp_exact (as_reg_fp h0 b) (as_reg_fp h0 c)) (I64.v (as_struct h0 a).mpfr_prec) rnd_mode (I32.v t) (as_fp h2 a);
+	mpfr_modifies_trans_lemma a h0 h1 h2;
+	t
+    end else begin
+        let t = mpfr_add1sp1_round a ap rnd_mode st in
+	let h2 = ST.get() in
+	mpfr_add1sp1_round_post_cond_lemma (add1sp_exact (as_reg_fp h0 b) (as_reg_fp h0 c)) (I64.v (as_struct h0 a).mpfr_prec) (as_normal_ h1 ({as_struct h1 a with mpfr_exp = st.bx})) (st.rb <> 0uL) (st.sb <> 0uL) rnd_mode (I32.v t) (as_fp h2 a);
+	mpfr_modifies_trans_lemma a h0 h1 h2;
+	t
+    end
+
+On fait l'arrondi
+*)
